Thread-local borrows.

lifetime.v
@@ -1,5 +1,5 @@
 From iris.program_logic Require Export viewshifts pviewshifts.
-From iris.program_logic Require Import invariants namespaces.
+From iris.program_logic Require Import invariants namespaces thread_local.
 From iris.prelude Require Import strings.
 From iris.proofmode Require Import invariants.
 
@@ -7,28 +7,26 @@ Definition lftN := nroot .@ "lft".
 
 Definition lifetime := positive.
 
-Axiom lifetimeG : ∀ (Λ:language) (Σ:gFunctors), Set.
+Axiom lifetimeG : ∀ (Σ:gFunctors), Set.
 Existing Class lifetimeG.
-Axiom lifetimeG_iris_inG : ∀ Λ Σ, lifetimeG Λ Σ → irisG Λ Σ.
-Existing Instance lifetimeG_iris_inG.
 
 (*** Definitions  *)
 
-Parameter lft : ∀ `{lifetimeG Λ Σ} (κ : lifetime), iProp Σ.
-Parameter lft_own : ∀ `{lifetimeG Λ Σ} (κ : lifetime) (q: Qp), iProp Σ.
-Parameter lft_dead : ∀ `{lifetimeG Λ Σ} (κ : lifetime), iProp Σ.
-Parameter lft_incl : ∀ `{lifetimeG Λ Σ} (κ κ' : lifetime), iProp Σ.
+Parameter lft : ∀ `{lifetimeG Σ} (κ : lifetime), iProp Σ.
+Parameter lft_own : ∀ `{lifetimeG Σ} (κ : lifetime) (q: Qp), iProp Σ.
+Parameter lft_dead : ∀ `{lifetimeG Σ} (κ : lifetime), iProp Σ.
+Parameter lft_incl : ∀ `{lifetimeG Σ} (κ κ' : lifetime), iProp Σ.
 Parameter lft_extract :
-  ∀ `{lifetimeG Λ Σ} (κ : lifetime) (P : iProp Σ), iProp Σ.
-Parameter lft_borrow : ∀ `{lifetimeG Λ Σ} (κ : lifetime) (P : iProp Σ), iProp Σ.
+  ∀ `{lifetimeG Σ} (κ : lifetime) (P : iProp Σ), iProp Σ.
+Parameter lft_borrow : ∀ `{lifetimeG Σ} (κ : lifetime) (P : iProp Σ), iProp Σ.
 Parameter lft_open_borrow :
-  ∀ `{lifetimeG Λ Σ} (κ : lifetime) (q:Qp) (P : iProp Σ), iProp Σ.
+  ∀ `{lifetimeG Σ} (κ : lifetime) (q:Qp) (P : iProp Σ), iProp Σ.
 Parameter lft_frac_borrow :
-  ∀ `{lifetimeG Λ Σ} (κ : lifetime) (P : Qp → iProp Σ), iProp Σ.
+  ∀ `{lifetimeG Σ} (κ : lifetime) (P : Qp → iProp Σ), iProp Σ.
 Parameter lft_pers_borrow :
-  ∀ `{lifetimeG Λ Σ} (κ : lifetime) (i : gname) (P : iProp Σ), iProp Σ.
+  ∀ `{lifetimeG Σ} (κ : lifetime) (i : gname) (P : iProp Σ), iProp Σ.
 Parameter lft_pers_borrow_own :
-  ∀ `{lifetimeG Λ Σ} (i : gname) (κ : lifetime), iProp Σ.
+  ∀ `{lifetimeG Σ} (i : gname) (κ : lifetime), iProp Σ.
 
 (*** Notations  *)
 
@@ -42,10 +40,10 @@ Notation "&{ κ } P" := (lft_borrow κ P)
 Notation "&frac{ κ } P" := (lft_frac_borrow κ P)
   (at level 20, right associativity) : uPred_scope.
 
-Section instances.
-  Context `{lifetimeG Λ Σ}.
+Section lft.
+  Context `{irisG Λ Σ, lifetimeG Σ}.
 
-  (*** PersitentP and TimelessP instances. *)
+  (*** PersitentP and TimelessP instances  *)
 
   Axiom lft_persistent : ∀ κ, PersistentP (lft κ).
   Global Existing Instance lft_persistent.
@@ -70,19 +68,14 @@ Section instances.
   Axiom lft_pers_borrow_own_timeless :
     ∀ i κ, TimelessP (lft_pers_borrow_own i κ).
   Global Existing Instance lft_pers_borrow_own_timeless.
-End instances.
 
-Section lft.
-
-  Context `{lifetimeG Λ Σ}.
-
-  (** Basic rules about lifetimes. *)
-  Axiom lft_begin :  ∀ `(nclose lftN ⊆ E), True ={E}=> ∃ κ, [κ]{1} ★ lft κ.
+  (** Basic rules about lifetimes  *)
+  Axiom lft_begin : ∀ `(nclose lftN ⊆ E), True ={E}=> ∃ κ, [κ]{1} ★ lft κ.
   (* TODO : Do we really need a full mask here ? *)
   Axiom lft_end : ∀ κ, lft κ ⊢ [κ]{1} ={⊤,∅}=★ ▷ |={∅,⊤}=> [†κ].
   Axiom lft_own_op : ∀ κ q1 q2, [κ]{q1} ★ [κ]{q2} ⊣⊢ [κ]{q1+q2}.
 
-  (** Creating borrows and using them. *)
+  (** Creating borrows and using them  *)
   Axiom lft_borrow_create :
     ∀ `(nclose lftN ⊆ E) κ P, lft κ ⊢ ▷ P ={E}=> &{κ}P ★ κ ∋ P.
   Axiom lft_borrow_split :
@@ -105,7 +98,7 @@ Section lft.
     ∀ `(nclose lftN ⊆ E) κ κ' P q',
       κ' ⊑ κ ⊢ &{κ}P ★ lft_open_borrow κ' q' (&{κ}P) ={E}=> [κ']{q'} ★ &{κ'}P.
 
-  (** Lifetime inclusion. *)
+  (** Lifetime inclusion  *)
   Axiom lft_mkincl :
     ∀ `(nclose lftN ⊆ E) κ κ' q, lft κ ⊢ &{κ'} [κ]{q} ={E}=> κ' ⊑ κ.
   Axiom lft_incl_refl : ∀ κ, True ⊢ κ ⊑ κ.
@@ -114,14 +107,14 @@ Section lft.
       [κ]{q} ={E}=> ∃ q', [κ']{q'} ★ ([κ']{q'} ={E}=★ [κ]{q}).
   Axiom lft_borrow_incl : ∀ κ κ' P, κ' ⊑ κ ⊢ &{κ}P → &{κ'}P.
 
-  (** Extraction. *)
+  (** Extraction  *)
   (* Axiom lft_extract_split : ∀ κ P Q, κ ∋ (P ★ Q) ={E}=> κ ∋ P ★ κ ∋ Q .*)
   Axiom lft_extract_combine :
     ∀ `(nclose lftN ⊆ E) κ P Q, κ ∋ P ★ κ ∋ Q ={E}=> κ ∋ (P ★ Q).
   Axiom lft_extract_out : ∀ `(nclose lftN ⊆ E) κ P, [†κ] ⊢ κ ∋ P ={E}=> ▷ P.
 
 
-  (** Fractured borrows. *)
+  (** Fractured borrows  *)
   (* TODO : I think an arbitrary mask is ok here. Not sure. *)
   Axiom lft_borrow_fracture : ∀ E κ φ, &{κ}(φ 1%Qp) ={E}=> &frac{κ}φ.
   Axiom lft_frac_borrow_open : ∀ `(nclose lftN ⊆ E) κ φ q,
@@ -129,7 +122,7 @@ Section lft.
      [κ]{q} ={E}=> ∃ q', ▷ φ q' ★ (▷ φ q' ={E}=★ [κ]{q}).
   Axiom lft_frac_borrow_incl : ∀ κ κ' φ, κ' ⊑ κ ⊢ &frac{κ}φ → &frac{κ'}φ.
 
-  (** Persistent borrows.  *)
+  (** Persistent borrows  *)
   (* TODO : Build all the other borrows from them. *)
   Axiom lft_borrow_persist :
     ∀ κ P, &{κ}P ⊣⊢ ∃ κ' i, κ ⊑ κ' ★ lft_pers_borrow κ' i P ★
@@ -139,49 +132,126 @@ Section lft.
       lft_pers_borrow κ i P ⊢ lft_pers_borrow_own i κ ★ [κ]{q} ={E}=> ▷ P ★
                                  (▷ P ={E}=★ lft_pers_borrow_own i κ ★ [κ]{q}).
 
+  (*** Derived lemmas  *)
+
+  Lemma lft_borrow_open' E κ P q :
+    nclose lftN ⊆ E →
+      &{κ}P ★ [κ]{q} ={E}=> ▷ P ★ (▷ P ={E}=★ &{κ}P ★ [κ]{q}).
+  Proof.
+    iIntros (?) "H". iVs (lft_borrow_open with "H") as "[HP Hopen]". done.
+    iVsIntro. iFrame. iIntros "HP".
+    iVs (lft_borrow_close with "[HP Hopen]"). done. by iFrame "HP". done.
+  Qed.
+
+  Lemma lft_mkincl' E κ κ' q :
+    nclose lftN ⊆ E →
+    lft κ ★ lft κ' ⊢ [κ]{q} ={E}=> κ' ⊑ κ ★ κ' ∋ [κ]{q}.
+  Proof.
+    iIntros (?) "[#Hκ#Hκ']!#?".
+    iVs (lft_borrow_create with "Hκ' [-]") as "[??]". done. by iFrame.
+    iFrame. by iApply (lft_mkincl with "Hκ [-]").
+  Qed.
+
 End lft.
 
-(*** Derived notions. *)
+(*** Derived notions  *)
 
-(** Shared borrows. *)
-Definition lft_shr_borrow `{lifetimeG Λ Σ} (κ : lifetime)
-                          (N : namespace) (P : iProp Σ) :=
+(** Shared borrows  *)
+Definition lft_shr_borrow `{irisG Λ Σ, lifetimeG Σ} (κ : lifetime)
+                           (N : namespace) (P : iProp Σ) :=
   (∃ κ' i, κ ⊑ κ' ★ lftN ⊥ N ★ lft_pers_borrow κ' i P
                   ★ inv N (lft_pers_borrow_own i κ'))%I.
-Instance lft_shr_borrow_persistent `{lifetimeG Λ Σ} κ N P :
-  PersistentP (lft_shr_borrow κ N P) := _.
 
 Notation "&shr{ κ | N } P" := (lft_shr_borrow κ N P)
   (at level 20, right associativity) : uPred_scope.
 
-Lemma lft_borrow_share `{lifetimeG Λ Σ} E κ P N :
-  lftN ⊥ N → &{κ}P ={E}=> &shr{κ|N}P.
-Proof.
-  iIntros (?) "HP".
-  iDestruct (lft_borrow_persist with "HP") as (κ' i) "(#?&#?&Hown)".
-  iExists κ', i. iVs (inv_alloc N E with "[Hown]").
-  by iIntros "!>"; iApply "Hown". by auto.
-Qed.
+Section shared_borrows.
+  Context `{irisG Λ Σ, lifetimeG Σ} (N : namespace).
 
-Lemma lft_shr_borrow_open `{lifetimeG Λ Σ} E κ P q N :
-  nclose N ⊆ E → nclose lftN ⊆ E →
-  &shr{κ|N}P ⊢ [κ]{q} ={E,E∖N}=> ▷P ★ (▷P ={E∖N,E}=★ [κ]{q}).
-Proof.
-  iIntros (??) "#HP!#Hκ".
-  iDestruct "HP" as (κ' i) "(#Hord&%&#Hpers&#Hinv)". iInv N as ">Hown" "Hclose".
-  iVs (lft_incl_trade with "Hord Hκ") as (q') "(Hκ'&Hclose')".
-    by auto using ndisj_subseteq_difference.
-  iVs (lft_pers_borrow_open with "Hpers [Hown Hκ']") as "[? Hclose'']".
-    by auto using ndisj_subseteq_difference. by iFrame.
-  iFrame. iIntros "!==>HP". iVs ("Hclose''" with "HP") as "[Hown Hκ]".
-  iVs ("Hclose'" with "Hκ"). iFrame. iApply "Hclose". auto.
-Qed.
+  Instance lft_shr_borrow_persistent κ P :
+    PersistentP (&shr{κ | N} P) := _.
 
-Lemma lft_shr_borrow_incl `{lifetimeG Λ Σ} κ κ' P N :
-  κ' ⊑ κ ⊢ &shr{κ|N}P → &shr{κ'|N}P.
-Proof.
-  iIntros "#Hord #HP". iDestruct "HP" as (κ0 i) "(#Hord'&%&#Hpers&#Hinv)".
-  iExists κ0, i. iSplit; last by eauto. iApply lft_incl_trans; eauto.
-Qed.
+  Lemma lft_borrow_share E κ P :
+    lftN ⊥ N → &{κ}P ={E}=> &shr{κ|N}P.
+  Proof.
+    iIntros (?) "HP".
+    iDestruct (lft_borrow_persist with "HP") as (κ' i) "(#?&#?&Hown)".
+    iExists κ', i. iVs (inv_alloc N E with "[Hown]").
+    by iIntros "!>"; iApply "Hown". by auto.
+  Qed.
+
+  Lemma lft_shr_borrow_open E κ P q :
+    nclose N ⊆ E → nclose lftN ⊆ E →
+    &shr{κ|N}P ⊢ [κ]{q} ={E,E∖N}=> ▷P ★ (▷P ={E∖N,E}=★ [κ]{q}).
+  Proof.
+    iIntros (??) "#HP!#Hκ".
+    iDestruct "HP" as (κ' i) "(#Hord&%&#Hpers&#Hinv)". iInv N as ">Hown" "Hclose".
+    iVs (lft_incl_trade with "Hord Hκ") as (q') "(Hκ'&Hclose')".
+      by auto using ndisj_subseteq_difference.
+    iVs (lft_pers_borrow_open with "Hpers [Hown Hκ']") as "[? Hclose'']".
+      by auto using ndisj_subseteq_difference. by iFrame.
+    iFrame. iIntros "!==>HP". iVs ("Hclose''" with "HP") as "[Hown Hκ]".
+    iVs ("Hclose'" with "Hκ"). iFrame. iApply "Hclose". auto.
+  Qed.
+
+  Lemma lft_shr_borrow_incl κ κ' P :
+    κ' ⊑ κ ⊢ &shr{κ|N}P → &shr{κ'|N}P.
+  Proof.
+    iIntros "#Hord #HP". iDestruct "HP" as (κ0 i) "(#Hord'&%&#Hpers&#Hinv)".
+    iExists κ0, i. iSplit; last by eauto. iApply lft_incl_trans; eauto.
+  Qed.
+End shared_borrows.
 
 Typeclasses Opaque lft_shr_borrow.
+
+(** Thread local borrows  *)
+
+Definition lft_tl_borrow `{irisG Λ Σ, lifetimeG Σ, thread_localG Σ}
+           (κ : lifetime) (tid : thread_id) (N : namespace) (P : iProp Σ) :=
+  (∃ κ' i, κ ⊑ κ' ★ lftN ⊥ N ★ lft_pers_borrow κ' i P
+                  ★ tl_inv tid N (lft_pers_borrow_own i κ'))%I.
+
+Notation "&tl{ κ | tid | N } P" := (lft_tl_borrow κ tid N P)
+  (at level 20, right associativity) : uPred_scope.
+
+Section tl_borrows.
+  Context `{irisG Λ Σ, lifetimeG Σ, thread_localG Σ}
+          (tid : thread_id) (N : namespace).
+
+  Instance lft_tl_borrow_persistent κ P :
+    PersistentP (&tl{κ|tid|N} P) := _.
+
+  Lemma lft_borrow_share_tl E κ P :
+    lftN ⊥ N → &{κ}P ={E}=> &tl{κ|tid|N}P.
+  Proof.
+    iIntros (?) "HP".
+    iDestruct (lft_borrow_persist with "HP") as (κ' i) "(#?&#?&Hown)".
+    iExists κ', i. iVs (tl_inv_alloc tid E N with "[Hown]").
+      by iIntros "!>"; iApply "Hown". by auto.
+  Qed.
+
+  Lemma lft_tl_borrow_open E F κ P q :
+    nclose lftN ⊆ E → nclose tlN ⊆ E → nclose N ⊆ F →
+    &tl{κ|tid|N}P ⊢ [κ]{q} ★ tl_own tid F ={E}=> ▷P ★ tl_own tid (F ∖ N) ★
+                     (▷P ★ tl_own tid (F ∖ N) ={E}=★ [κ]{q} ★ tl_own tid F).
+  Proof.
+    iIntros (???) "#HP!#[Hκ Htlown]".
+    iDestruct "HP" as (κ' i) "(#Hord&%&#Hpers&#Hinv)".
+    iVs (tl_inv_open with "Hinv Htlown") as "(>Hown&Htlown&Hclose)"; try done.
+    iVs (lft_incl_trade with "Hord Hκ") as (q') "(Hκ'&Hclose')". done.
+    iVs (lft_pers_borrow_open with "Hpers [Hown Hκ']") as "[? Hclose'']".
+      done. by iFrame.
+    iFrame. iIntros "!==>[HP Htlown]". iVs ("Hclose''" with "HP") as "[Hown Hκ]".
+    iVs ("Hclose'" with "Hκ"). iFrame. iApply "Hclose". by iFrame.
+  Qed.
+
+  Lemma lft_tl_borrow_incl κ κ' P :
+    κ' ⊑ κ ⊢ &tl{κ|tid|N}P → &tl{κ'|tid|N}P.
+  Proof.
+    iIntros "#Hord #HP". iDestruct "HP" as (κ0 i) "(#Hord'&%&#Hpers&#Hinv)".
+    iExists κ0, i. iSplit; last by eauto. iApply lft_incl_trans; eauto.
+  Qed.
+
+End tl_borrows.
+
+Typeclasses Opaque lft_tl_borrow.
